---
title: "Propositional Logic"
parent: "Discrete Mathematics"
subject: "Computer Science"
type: "Semester"
id: 2401281130
---

# Proposition

A proposition is a declarative statement which is either **true** or **false**. For example, considering the statement: _New Delhi is the capital of India_, is a proposition. On the other hand, considering: $x+2=10$, is not a proposition because the value of $x$ is unknown, therefore, cannot be stated whether, it is true or false.

---

# Propositional Operators

## Negation

Representation: $\sim,\lnot$

If $p$ is the proposition, then the negation of $p$ is denoted by $\sim p$, and it simply reverses the truth value of $p$.

E.g.:

$p:\textnormal{It is cold today}
$

$\sim p:\textnormal{It is not cold today}$

#### Truth table:

| $p$ | $\sim p$ |
| --- | -------- |
| T   | F        |
| F   | T        |

## Conjugation

Representation: $\wedge$

For any two proposition, $p$ and $q$, the conjunction is denoted by $p\wedge q$, and it gives the true value when both $p$ and $q$ are true.

E.g.:

$p:\textnormal{It is cold today}$

$q:\textnormal{It is Friday}$

$p\wedge q:\textnormal{It is cold today and it is Friday}$

#### Truth table:

| $p$ | $q$ | $p\wedge q$ |
| --- | --- | ----------- |
| T   | T   | T           |
| T   | F   | F           |
| F   | T   | F           |
| F   | F   | F           |

## Disjunction

Representation: $\vee$

For any two proposition $p$, and $q$, the disjunction is denoted by $p\vee q$, and gives the true value if either of them or both are true.

E.g.:

$p:\textnormal{It is cold today}$

$q:\textnormal{It is Friday}$

$p\vee q:\textnormal{Either it is cold today or it is Friday}$

#### Truth table:

| $p$ | $q$ | $p\vee q$ |
| --- | --- | --------- |
| T   | T   | T         |
| T   | F   | T         |
| F   | T   | T         |
| F   | F   | F         |

## Implication

Representation: $\to$

For any two proposition $p$ and $q$, the statement if $p$ then $q$ is called an implication and it is denoted by $p\to q$. It gives false when $p$ is true and $q$ is false, otherwise it is true.

E.g.:

$p:\textnormal{It is cold today}$

$q:\textnormal{It is Friday}$

$p\to q:\textnormal{If it is cold today then it is Friday}$

#### Truth table

| $p$ | $q$ | $p\to q$ |
| --- | --- | -------- |
| T   | T   | T        |
| T   | F   | F        |
| F   | T   | T        |
| F   | F   | T        |

## Bi

Representation: $\leftrightarrow$

For any two proposition $p$ and $q$, the statement $p$, _iff._, $q$ is called biconditional, and is denoted by $p\leftrightarrow q$. It gives true value when both $p$ and $q$ have the same value.

E.g.:

$q:\textnormal{It is cold today}$

$q:\textnormal{It is Friday}$

$p\leftrightarrow q:\textnormal{It is cold today iff. it is Friday}$

#### Truth table

| $p$ | $q$ | $p\leftrightarrow q$ |
| --- | --- | -------------------- |
| T   | T   | T                    |
| T   | F   | F                    |
| F   | T   | F                    |
| F   | F   | T                    |

---

#### Example 1: Express the following statement in propositional logic:

$$
\textnormal{It is Saturday and I am not going to college}
$$

Solution:

$p:\textnormal{It is Saturday}$

$q:\textnormal{I am going to college}$

Well formed formula (WFF): $p\wedge\sim q$

#### Example 2: Express the following statement in propositional logic:

$$
\textnormal{Either it is hot today or I am at home}
$$

Solution:

$p:\textnormal{It is hot today}$

$q:\textnormal{I am at home}$

Well formed formula (WFF): $p\vee q$

#### Example 3: Express the following statement in propositional logic:

$$
3+4\ne6\textnormal{ and C.S. class will not be held}
$$

Solution:

$p:3+4=6$

$q:\textnormal{C.S. class will be held}$

Well formed formula (WFF): $\sim p\wedge\sim q$

#### Example 4: Draw the truth table for $(\sim p\wedge q)\wedge \sim r$.

| $p$ | $q$ | $r$ | $\sim p\wedge q$ | $(\sim p\wedge q)\wedge \sim r)$ |
| --- | --- | --- | ---------------- | -------------------------------- |
| T   | T   | T   | F                | F                                |
| T   | T   | F   | F                | F                                |
| T   | F   | T   | F                | F                                |
| T   | F   | F   | F                | F                                |
| F   | T   | T   | T                | F                                |
| F   | T   | F   | T                | T                                |
| F   | F   | T   | F                | F                                |
| F   | F   | F   | F                | F                                |

#### Example 5: Check the equivalence for the following:

$$
p\to(q\to r)\cong(p\wedge q)\to r
$$

Solution:

| $p$ | $q$ | $r$ | $q\to r$ | $p\to(q\to r)$ | $p\wedge q$ | $(p\wedge q)\to r$ |
| --- | --- | --- | -------- | -------------- | ----------- | ------------------ |
| T   | T   | T   | T        | T              | T           | T                  |
| T   | T   | F   | F        | F              | T           | F                  |
| T   | F   | T   | T        | T              | F           | T                  |
| T   | F   | F   | T        | T              | F           | T                  |
| F   | T   | T   | T        | T              | F           | T                  |
| F   | T   | F   | F        | T              | F           | T                  |
| F   | F   | T   | T        | T              | F           | T                  |
| F   | F   | F   | T        | T              | F           | T                  |

From the truth table, it can be concluded that:

$$
p\to(q\to r)\cong(p\wedge q)\to r
$$

Implication and bicondition can be further be simplifed as:

$$
p\rightarrow q=\sim p\vee q
$$

$$
p\leftrightarrow q=(p\rightarrow q)\wedge(q\rightarrow p)=(\sim p\vee q)\wedge(\sim q\vee p)
$$

---

# Laws for propositional logic

Following are the laws for propositional logic:

1. **Idempotent law:**
   - $p\wedge p=p$
   - $p\vee p=p$
2. **Commutative law:**
   - $p\vee q=q\vee p$
   - $p\wedge q=q\wedge p$
3. **Associative law:**
   - $(p\vee q)\vee r=p\vee(q\vee r)$
   - $(p\wedge q)\wedge r=p\wedge(q\wedge r)$
4. **Distributive law:**
   - $p\wedge(q\vee r)=(p\wedge q)\vee(p\wedge r)$
   - $p\vee(q\wedge r)=(p\vee q)\wedge(p\vee r)$
5. **Identity law:**
   - $p\vee T=T$
   - $p\wedge T=p$
   - $p\vee F=p$
   - $p\wedge F=F$
6. **De-morgan's law:**
   - $\sim(p\vee q)=\sim p\wedge\sim q$
   - $\sim(p\wedge q)=\sim p\vee\sim q$
7. **Involution law:**
   - $\sim(\sim p)=p$
8. **Compliment law:**
   - $p\vee\sim p=T$
   - $p\wedge\sim p=F$
9. **Contrapositive law:**
   - $p\rightarrow q=\sim q\rightarrow\sim p$

---

# Conditions for compound statements

## Tautology

We define a term, **tautology** for a compound statement such that its truth value is **always true** for all possible combinations. For example:

$$
(p\wedge q)\rightarrow(p\vee q)
$$

Truth table:

| p   | q   | $p\wedge q$ | $p\vee q$ | $(p\wedge q)\rightarrow(p\vee q)$ |
| --- | --- | ----------- | --------- | --------------------------------- |
| T   | T   | T           | T         | T                                 |
| T   | F   | F           | T         | T                                 |
| F   | T   | F           | T         | T                                 |
| F   | F   | F           | F         | T                                 |

Since, all values for the compound statemnet is true, it is tautogenic.

## Contradiction

We define a term, **contradiction** for a compound statement such that its truth value is **always false** for all possible combinations. For example:

$$
\sim(\sim(p\wedge q)\leftrightarrow(\sim p\vee\sim q))\\
=\sim((\sim(p\wedge q)\rightarrow(\sim p\vee\sim q))\wedge((\sim p\vee\sim q)\rightarrow(\sim(p\wedge q)))\\
$$

We know, as per De-morgan's theorem: $\sim p\vee\sim q=\sim(p\wedge q)$

$$
\therefore \sim((\sim(p\wedge q)\rightarrow(\sim p\vee\sim q))\wedge((\sim p\vee\sim q)\rightarrow\sim(p\wedge q)))\\
=\sim((\sim(p\wedge q)\rightarrow\sim(p\wedge q))\wedge(\sim(p\wedge q)\rightarrow\sim(p\wedge q)))\\
$$

We know: $p\rightarrow p=T$. Similarly, $\sim(p\wedge q)\rightarrow\sim(p\wedge q)=T$

$$
\therefore \sim((\sim(p\wedge q)\rightarrow\sim(p\wedge q))\wedge(\sim(p\wedge q)\rightarrow\sim(p\wedge q)))\\
=\sim(T\wedge T)=\sim T=F
$$

Since the final result is $F$, therefore the compound statement is contradictive.

## Contigency

A compound statement that is neither a tortology nor a contradiction is called contigency. For example: $p\vee q$

#### Example 6: $\sim p\rightarrow \sim q\cong \sim q\vee p$. Prove the equivalence.

$$
\textnormal{LHP}\\
=\sim p\rightarrow\sim q\\
=\sim(\sim p)\vee \sim q
$$

As: $p\to q=\sim p\vee q$, and since $\sim(\sim p)=p$

$$
\therefore \sim(\sim p)\vee \sim q\\
=p\vee\sim q=\sim q\vee p=\textnormal{RHP}
$$

Therefore, $\sim p\rightarrow \sim q\cong \sim q\vee p$.

#### Example 7: Show that $(p\wedge q)\to(p\vee q)$ is tautogenic.

$$
(p\wedge q)\to(p\vee q)\\
=\sim(p\wedge q)\vee p\vee q\\
=\sim p \vee \sim q\vee p \vee q\\
=(\sim p\vee p)\vee(\sim q\vee q)\\
=T\vee T=T=\textnormal{RHP}
$$

Therefore, the given proposition is tautogenic

#### Example 8: Show that $p\to(p\wedge(q\to p))$ is tautogenic.

$$
p\to(p\wedge(q\to p))\\
=p\to(p\wedge(\sim q\vee p))\\
=\sim p\vee(p\wedge(\sim q\vee p))\\
=(\sim p\vee p)\wedge(\sim p\vee \sim q \vee p)\\
=T\wedge(T\vee\sim q)\\
=T\wedge T=T
$$

Therefore, the given proposition is tautogenic.

#### Problem 1: Prove the equivalence of $p\to(q\to r)\cong(p\wedge q)\to r$.
